Re-write algorithm without shortcuts.

Cslib/Computability/Machines/MultiTapeTuring/GraphReachability.lean
@@ -32,29 +32,28 @@ def reachable(a, b, t, r):
   if t = 0:
     return r(a, b)
   else:
+    result = False
     for c in vertices:
-      if reachable(a, c, t - 1, r) and reachable(c, b, t - 1, r):
-        return True
-    return False
+      result |= reachable(a, c, t - 1, r) and reachable(c, b, t - 1, r)
+    return result
 
 Until we have a generic mechanism for recursion, let's translate this into a program that
 uses "goto", and every variable is a stack:
 
 def reachable(a, b, t, edge):
-  result = 0
   pc = [:fun_start]
   while !pc.is_empty():
     match pc.pop()
     | :fun_start =>
       if t = 0:
-        result = edge(a, b)
+        result.push(edge(a, b))
       else:
         c.push(0)
+        result.push(0)
         pc.push(:loop_start)
     | :loop_start =>
       if c.top() = num_vertices:
         c.pop()
-        result = 0
       else:
         a.push(a.top())
         b.push(c.top())
@@ -64,25 +63,16 @@ def reachable(a, b, t, edge):
     | :after_first_rec =>
         a.pop()
         b.pop()
-        t = t + 1
-        if result == 1:
-          a.push(c.top())
-          b.push(b.top())
-          t = t - 1
-          pc.push(:after_second_rec)
-          pc.push(:fun_start)
-        else:
-          result = 0
-          pc.push(:loop_continue)
+        -- we keep the result of the first recursive call.
+        a.push(c.top())
+        b.push(b.top())
+        pc.push(:after_second_rec)
+        pc.push(:fun_start)
     | :after_second_rec =>
         a.pop()
         b.pop()
         t = t + 1
-        if result == 1:
-          c.pop()
-        else:
-          pc.push(:loop_continue)
-    | :loop_continue =>
+        result.push(result.pop() ∨ result.pop() ∨ result.pop())
         c.top() += 1
         pc.push(:loop_start)
   -- cleanup
@@ -111,29 +101,6 @@ abbrev l_afterFirstRec := dya 3
 abbrev l_afterSecondRec := dya 4
 abbrev l_loopContinue := dya 5
 
--- if t = 0:
---   result = edge(a, b)
--- else:
---   c.push(0)
---   pc.push(:loop_start)
-
-def funStart (edge : MultiTapeTM tapeCount (WithSep OneTwo)) :=
-  ite t (push c [] <;> push pc l_loopStart) edge
-
-@[simp]
-lemma funStart_eval_list
-  (tapes : Fin tapeCount → List (List OneTwo))
-  (edge : MultiTapeTM tapeCount (WithSep OneTwo)) :
-  (funStart edge).eval_list tapes =
-    if (tapes t).headD [] = [] then
-      (edge.eval_list tapes)
-    else
-      .some (Function.update (Function.update tapes c ([] :: (tapes c)))
-        pc (l_loopStart :: (tapes pc))) := by
-  simp [funStart]
-
-def infiniteLoop {α : Type} {k : ℕ} : MultiTapeTM k (WithSep α) := sorry
-
 public def eqLit {k : ℕ}
   (q : Fin (k + 3))
   (w : List OneTwo)
@@ -158,71 +125,7 @@ public theorem eqLit_eval_list {k : ℕ} {q s aux : Fin (k + 3)} {w : List OneTw
   have h_neq : q ≠ aux := Function.Injective.ne h_inj (a₁ := 0) (a₂ := 1) (by grind)
   grind
 
--- | :loop_start =>
--- if c.top() = num_vertices:
---   c.pop()
---   result = 0
--- else:
---   a.push(a.top())
---   b.push(c.top())
---   t = t - 1
---   pc.push(:after_first_rec)
---   pc.push(:fun_start)
-
-def loopStart (maxConfig : List OneTwo) :=
-  eqLit c maxConfig mainAux <;>
-    ite mainAux
-      (pop mainAux <;> pop c <;> push result [])
-      (pop mainAux <;> duplicate a <;> copy c b <;>
-        dec t mainAux (by decide) <;> push pc l_afterFirstRec <;> push pc l_funStart)
-
--- TODO this simp lemma is probably not really needed, because the proof is just `simp [loopStart]`
-
--- @[simp]
--- lemma loopStart_eval_list
---   (maxConfig : List OneTwo)
---   (loopStart maxConfig).eval_list tapes = .some sorry := by
---   simp [loopStart]
---   sorry
-
--- | :after_first_rec =>
---     a.pop()
---     b.pop()
---     t = t + 1
---     if result == 1:
---       a.push(c.top())
---       b.push(b.top())
---       t = t - 1
---       pc.push(:after_second_rec)
---       pc.push(:fun_start)
---     else:
---       result = 0
---       pc.push(:loop_continue)
-
-def afterFirstRec :=
-  pop a <;> pop b <;> succ t <;> ite result
-    (duplicate c <;> duplicate b <;> dec t mainAux (by decide) <;>
-      push pc l_afterSecondRec <;> push pc l_funStart)
-    (pop result <;> push result [] <;> push pc l_loopContinue)
-
--- | :after_second_rec =>
---     a.pop()
---     b.pop()
---     t = t + 1
---     if result == 1:
---       c.pop()
---     else:
---       pc.push(:loop_continue)
-
-def afterSecondRec :=
-  pop a <;> pop b <;> succ t <;> ite result (pop c) (push pc l_loopContinue)
-
--- | :loop_continue =>
---     c.top() += 1
---     pc.push(:loop_start)
-
-def loopContinue := succ c <;> push pc l_loopStart
-
+@[simp]
 public def iteLit {k : ℕ}
   (i : Fin (k + 3))
   (w : List OneTwo)
@@ -233,45 +136,81 @@ public def iteLit {k : ℕ}
     eqLit i w (aux + 1) aux (h_inj := by intro x y; grind) <;>
       ite (aux + 1) (pop (aux + 1) <;> tm₁) (pop (aux + 1) <;> tm₂)
 
--- TODO not sure if this simp lemma is needed. We can also put @[simp] at iteLit instead.
+@[simp]
+public def combineOr {k : ℕ} (i : Fin k) :
+  MultiTapeTM k (WithSep OneTwo) :=
+    ite i
+      (pop i <;> pop i <;> push i [OneTwo.one])
+      (pop i <;>
+        ite i
+          (pop i <;> push i [OneTwo.one])
+          (pop i <;> push i []))
+
+
+-- | :fun_start =>
+-- if t = 0:
+--   result.push(edge(a, b))
+-- else:
+--   c.push(0)
+--   result.push(0)
+--   pc.push(:loop_start)
 
 @[simp]
-lemma itLit_eval_list {k : ℕ}
-  (i : Fin (k + 3))
-  (w : List OneTwo)
-  (aux : Fin (k + 3))
-  (tm₁ tm₂ : MultiTapeTM (k + 3) (WithSep OneTwo))
-  (h_inj : [i, aux, aux + 1].get.Injective)
-  (tapes : Fin (k + 3) → List (List OneTwo)) :
-  (iteLit i w aux tm₁ tm₂ h_inj).eval_list tapes =
-      if (tapes i).headD [] = w then tm₁.eval_list tapes else tm₂.eval_list tapes := by
-  simp [iteLit]
+def funStart (edge : MultiTapeTM tapeCount (WithSep OneTwo)) :=
+  ite t (push c [] <;> push result [] <;> push pc l_loopStart) edge
 
-public def matchCombine {k : ℕ}
-  (i : Fin (k + 3)) (aux : Fin (k + 3)) (h_inj : [i, aux, aux + 1].get.Injective)
-  (branches : List ((List OneTwo) × (MultiTapeTM (k + 3) (WithSep OneTwo)))) :
-  MultiTapeTM (k + 3) (WithSep OneTwo) :=
-  match branches with
-  | [] => infiniteLoop
-  | (w, tm) :: branches =>
-      eqLit i w aux (aux + 1) (h_inj := by sorry /- use swap on h_inj? -/) <;>
-        ite aux (pop aux <;> tm) (pop aux <;> matchCombine i aux (by intro x y; grind) branches)
+-- | :loop_start =>
+-- if c.top() = num_vertices:
+--   c.pop()
+-- else:
+--   a.push(a.top())
+--   b.push(c.top())
+--   t = t - 1
+--   pc.push(:after_first_rec)
+--   pc.push(:fun_start)
 
+@[simp]
+def loopStart (maxConfig : List OneTwo) :=
+  iteLit c maxConfig mainAux
+    (pop c)
+    (duplicate a <;> copy c b <;>
+      dec t mainAux (by decide) <;> push pc l_afterFirstRec <;> push pc l_funStart)
+
+-- | :after_first_rec =>
+-- a.pop()
+-- b.pop()
+-- -- we keep the result of the first recursive call.
+-- a.push(c.top())
+-- b.push(b.top())
+-- pc.push(:after_second_rec)
+-- pc.push(:fun_start)
+
+@[simp]
+def afterFirstRec :=
+  pop a <;> pop b <;> copy c a <;> duplicate b <;>
+    push pc l_afterSecondRec <;> push pc l_funStart
+
+-- | :after_second_rec =>
+-- a.pop()
+-- b.pop()
+-- t = t + 1
+-- result.push(result.pop() ∨ result.pop() ∨ result.pop())
+-- c.top() += 1
+-- pc.push(:loop_start)
+
+@[simp]
+def afterSecondRec :=
+  pop a <;> pop b <;> succ t <;>
+    combineOr result <;> combineOr result <;> succ c <;> push pc l_loopStart
+
+
+@[simp]
 def innerLoop (edge : MultiTapeTM tapeCount (WithSep OneTwo)) (maxConfig : List OneTwo) :
     MultiTapeTM tapeCount (WithSep OneTwo) :=
   iteLit pc l_funStart mainAux (pop pc <;> funStart edge)
     (iteLit pc l_loopStart mainAux (pop pc <;> loopStart maxConfig)
       (iteLit pc l_afterFirstRec mainAux (pop pc <;> afterFirstRec)
-        (iteLit pc l_afterSecondRec mainAux (pop pc <;> afterSecondRec)
-          (pop pc <;> loopContinue))))
-
-lemma innerLoop_eval_list
-  (edge : MultiTapeTM tapeCount (WithSep OneTwo))
-  (maxConfig : List OneTwo)
-  (tapes : Fin tapeCount → List (List OneTwo)) :
-  (innerLoop edge maxConfig).eval_list tapes = sorry := by
-  simp [innerLoop, loopStart, afterFirstRec, afterSecondRec, loopContinue]
-  sorry
+        (pop pc <;> afterSecondRec)))
 
 lemma relatesInStepsExp {α : Type}
   (r : α → α → Prop)
@@ -285,6 +224,14 @@ lemma relatesInStepsExp {α : Type}
 def finiteRel (r : (List OneTwo) → (List OneTwo) → Prop) (max : ℕ) : Prop :=
   ∀ a b, r a b → (dya_inv a < max ∧ dya_inv b < max)
 
+lemma finiteRel_apply₁ {r : (List OneTwo) → (List OneTwo) → Prop} {max : ℕ}
+  (h_finite : finiteRel r max) {a b : List OneTwo} (h_r : r a b) :
+    dya_inv a < max := (h_finite a b h_r).1
+
+lemma finiteRel_apply₂ {r : (List OneTwo) → (List OneTwo) → Prop} {max : ℕ}
+  (h_finite : finiteRel r max) {a b : List OneTwo} (h_r : r a b) :
+    dya_inv b < max := (h_finite a b h_r).2
+
 def edge_semantics
   (r : (List OneTwo) → (List OneTwo) → Prop)
   (h_r_dec : ∀ x y, Decidable (r x y))
@@ -294,26 +241,6 @@ def edge_semantics
     Function.update tapes result ([.one] :: (tapes result))
   else
     Function.update tapes result ([] :: (tapes result)))
-
-lemma inner_loop_induction_basis
-  (r : (List OneTwo) → (List OneTwo) → Prop)
-  (h_r_dec : ∀ x y, Decidable (r x y))
-  (max : ℕ)
-  (edge : MultiTapeTM tapeCount (WithSep OneTwo))
-  (h_edge_semantics : edge_semantics r h_r_dec edge)
-  (tapes : Fin tapeCount → List (List OneTwo))
-  (h_pc : (tapes pc).head?.getD [] = l_funStart)
-  (h_t : (tapes t).head?.getD [] = []) :
-  (innerLoop edge (dya max)).eval_list tapes = .some
-    (Function.update (Function.update tapes
-      pc (tapes pc).tail)
-      result (if r ((tapes a).headD []) ((tapes b).headD []) then
-        [.one] :: (tapes result)
-      else
-        [] :: (tapes result))) := by
-  unfold edge_semantics at h_edge_semantics
-  simp [innerLoop, h_pc, h_t, h_edge_semantics]
-  grind
 
 lemma inner_loop_halts_on_lists
   {r : (List OneTwo) → (List OneTwo) → Prop}
@@ -325,8 +252,8 @@ lemma inner_loop_halts_on_lists
   intro tapes
   apply MultiTapeTM.HaltsOnLists_of_eval_list
   unfold edge_semantics at h_edge_semantics
-  simp [innerLoop, loopStart, afterFirstRec, afterSecondRec, loopContinue, h_edge_semantics]
-  split_ifs -- todo use <;>
+  simp [h_edge_semantics]
+  split_ifs
   · simp
   · simp
   · simp
@@ -334,67 +261,97 @@ lemma inner_loop_halts_on_lists
   · simp
   · simp
   · simp
-  · simp
+    split_ifs
+    · simp
+    · simp
   · simp
   · simp
 
-def reachability (edge : MultiTapeTM tapeCount (WithSep OneTwo)) (maxConfig : List OneTwo) :
-    MultiTapeTM tapeCount (WithSep OneTwo) :=
-  doWhile pc (innerLoop edge maxConfig)
+def reachability
+  (edge : MultiTapeTM tapeCount (WithSep OneTwo))
+  (maxConfig : List OneTwo)
+  (x y : List OneTwo)
+  (t_val : ℕ) :=
+  push a x <;> push b y <;> push t (dya t_val) <;> push pc [] <;> push pc l_funStart <;>
+    doWhile pc (innerLoop edge maxConfig) <;>
+    pop t <;> pop a <;> pop b
+
+@[simp]
+def iter_count_bound (max : ℕ) (t : ℕ) : ℕ := match t with
+  | .zero => 1
+  | .succ t' => 2 + max * (3 + 2 * iter_count_bound max t')
+
+@[simp]
+noncomputable def innerLoopFun
+  {r : (List OneTwo) → (List OneTwo) → Prop}
+  {h_r_dec : ∀ x y, Decidable (r x y)}
+  (max : ℕ)
+  {edge : MultiTapeTM tapeCount (WithSep OneTwo)}
+  (h_edge_semantics : edge_semantics r h_r_dec edge) :=
+    (innerLoop edge (dya max)).eval_list_tot (inner_loop_halts_on_lists h_edge_semantics)
+
+-- TODO continue here: prove this theorem by induction.
+lemma loop_semantics
+  {r : (List OneTwo) → (List OneTwo) → Prop}
+  {h_r_dec : ∀ x y, Decidable (r x y)}
+  (h_rs_dec : ∀ x y t, Decidable (Relation.RelatesInSteps r x y t))
+  {max : ℕ}
+  (h_finite : finiteRel r max)
+  {edge : MultiTapeTM tapeCount (WithSep OneTwo)}
+  (h_edge_semantics : edge_semantics r h_r_dec edge)
+  (tapes : Fin tapeCount → List (List OneTwo))
+  (h_pc_funStart : (tapes pc).head?.getD [] = l_funStart) :
+    (innerLoopFun max h_edge_semantics)^[iter_count_bound max (dya_inv ((tapes t).headD []))]
+        tapes = Function.update (Function.update tapes
+      pc (tapes pc).tail)
+      result (
+        if Relation.RelatesInSteps r ((tapes a).headD []) ((tapes b).headD [])
+              (Nat.pow 2 (dya_inv ((tapes t).headD []))) then
+          [.one] :: (tapes result)
+        else
+          [] :: (tapes result)) ∧
+      ∀ n' < iter_count_bound max (dya_inv ((tapes t).headD [])),
+        (((innerLoopFun max h_edge_semantics)^[n'] tapes) pc).length ≥ (tapes pc).length := by
+  induction h_t : (dya_inv ((tapes t).headD [])) generalizing tapes with
+    | zero =>
+      have h_t_dya : (tapes t).head?.getD [] = dya 0 := by rw [← h_t]; simp
+      unfold edge_semantics at h_edge_semantics
+      simp [h_edge_semantics, h_pc_funStart, h_t_dya, Relation.RelatesInSteps.single_iff]
+      split
+      · simp
+      · simp
+    | succ t_val ih =>
+      by_cases h_rel : Relation.RelatesInSteps r
+          ((tapes a).headD []) ((tapes b).headD []) (Nat.pow 2 (t_val + 1))
+      · simp only [h_rel]
+        simp
+        obtain ⟨c, h_c_rel⟩ :=
+          (relatesInStepsExp r ((tapes a).headD []) ((tapes b).headD []) t_val).mp h_rel
+        have h_c_le : dya_inv c < max := by sorry
+
+        sorry
+      · sorry
+
 
 theorem reachability_eval_list
-  (r : (List OneTwo) → (List OneTwo) → Prop)
-  (h_r_dec : ∀ x y, Decidable (r x y))
+  {r : (List OneTwo) → (List OneTwo) → Prop}
+  {h_r_dec : ∀ x y, Decidable (r x y)}
   (h_rs_dec : ∀ x y t, Decidable (Relation.RelatesInSteps r x y t))
-  (max : ℕ)
+  {max : ℕ}
   (h_finite : finiteRel r max)
-  (edge : MultiTapeTM tapeCount (WithSep OneTwo))
+  {edge : MultiTapeTM tapeCount (WithSep OneTwo)}
   (h_edge_semantics : edge_semantics r h_r_dec edge)
-  (t_val : ℕ)
-  (a_val b_val : List OneTwo)
-  (tapes : Fin tapeCount → List (List OneTwo)) :
-  (push a a_val <;> push b b_val <;> push t (dya t_val) <;>
-    reachability edge (dya max)).eval_list tapes = .some (Function.update tapes result (
+  {t_val : ℕ}
+  {a_val b_val : List OneTwo}
+  {tapes : Fin tapeCount → List (List OneTwo)} :
+  (reachability edge (dya max) a_val b_val t_val).eval_list tapes = .some (Function.update tapes
+    result (
       if Relation.RelatesInSteps r a_val b_val t_val then
         [.one] :: (tapes result)
       else
         [] :: (tapes result))) := by
   simp [reachability]
-  rw [doWhile_eval_list (inner_loop_halts_on_lists h_edge_semantics)]
-  simp
   sorry
-
-lemma induction_step
-  (r : (List OneTwo) → (List OneTwo) → Prop)
-  (h_r_dec : ∀ x y, Decidable (r x y))
-  (max : ℕ)
-  (edge : MultiTapeTM tapeCount (WithSep OneTwo))
-  (h_edge_semantics : edge_semantics r h_r_dec edge)
-  (tapes : Fin tapeCount → List (List OneTwo))
-  (h_pc : (tapes pc).head?.getD [] = l_funStart)
-  (t_val : ℕ)
-  (h_t : (tapes t).head?.getD [] = dya t_val.succ)
-  (h_ih : ∀ tapes',
-    (tapes' pc).head?.getD [] = l_funStart →
-    (tapes' t).head?.getD [] = dya t_val →
-    (innerLoop edge (dya max)).eval_list tapes' = .some
-      (Function.update (Function.update tapes'
-        pc (tapes' pc).tail)
-        result (if r ((tapes' a).headD []) ((tapes' b).headD []) then
-          [.one] :: (tapes' result)
-        else
-          [] :: (tapes' result))) →
-   :
-  (innerLoop edge (dya max)).eval_list tapes = .some
-    (Function.update (Function.update tapes
-      pc (tapes pc).tail)
-      result (if r ((tapes a).headD []) ((tapes b).headD []) then
-        [.one] :: (tapes result)
-      else
-        [] :: (tapes result))) := by
-  unfold edge_semantics at h_edge_semantics
-  simp [innerLoop, h_pc, h_t, h_edge_semantics]
-  grind
 
 
 end Routines
